coq/theories/automation/RelCompilerCommons.v
@@ -1,0 +1,3 @@
+From Ltac2 Require Import Ltac2.
+
+Ltac2 mutable debug_relcompile := false.
