coq/theories/automation/ToLowerable.v
@@ -1,13 +1,13 @@
-From Ltac2 Require Import Ltac2 Constr Std RedFlags.
+From Ltac2 Require Import Ltac2 Constr Std RedFlags Printf.
 From impboot Require Import utils.Core.
 From impboot Require Import utils.AppList.
 From coqutil Require Import dlet.
 From coqutil Require Import Word.Interface.
-From impboot Require Import
-  commons.CompilerUtils
-  automation.ToANF.
+From impboot Require Import commons.CompilerUtils.
+From impboot.functional Require Import FunSemantics FunValues.
 
-(* rewrite every N.mul to mul_N call and every Nat.mul to nat_mul call *)
+Open Scope list_scope.
+Open Scope nat.
 
 Lemma dlet_spec: forall {A B: Type} (a: A) (f: A -> B),
   let/d x := a in f x = let x := a in f x.
@@ -15,54 +15,60 @@ Proof.
   intros; reflexivity ().
 Qed.
 
-Lemma split_string: forall {A} (c1 c2 c3 c4 c5: ascii) (s: string) (k: string -> A),
-  (let/d str1 := String c1 (String c2 (String c3 (String c4 (String c5 s)))) in k str1) =
-  let/d str_front := String c1 (String c2 (String c3 (String c4 EmptyString))) in
-  let/d str_rest := String c5 s in
-  let/d str1 := append str_front str_rest in
-  k str1.
-Proof.
-  intros; reflexivity ().
-Qed.
-
-Lemma split_list: forall {A B} (e1 e2 e3 e4 e5: A) (l: list A) (k: list A -> B),
-  (let/d l1 := e1 :: e2 :: e3 :: e4 :: e5 :: l in k l1) =
-  let/d l_front := e1 :: e2 :: e3 :: e4 :: [] in
-  let/d l_rest := e5 :: l in
-  let/d l1 := l_front ++ l_rest in
-  k l1.
-Proof.
-  intros; reflexivity ().
-Qed.
+Ltac2 lower_match_constr (c: constr): unit :=
+  try (match! c with
+  | context [ N.mul _ _ ] =>
+    rewrite <- mul_N_spec
+  | context [ Nat.mul _ _ ] =>
+    rewrite <- mul_nat_spec
+  | context [ append _ _ ] =>
+    rewrite <- string_append_spec
+  | context [ List.app _ _ ] =>
+    rewrite <- list_append_spec
+  | context [ List.length _ ] =>
+    rewrite <- list_length_spec
+  | context [ dlet (String ?c1 (String ?c2 (String ?c3 (String ?c4 (String ?c5 ?str))))) ?f ] =>
+    let prfx := constr:(String $c1 (String $c2 (String $c3 (String $c4 EmptyString)))) in
+    let sfx := constr:(String $c5 $str) in
+    let new_constr := constr:(
+      let/d prfx := $prfx in
+      let/d sfx := $sfx in
+      dlet (append prfx sfx) $f
+    ) in
+    (* TODO: should use change (change old with new), but it doesn't sometimes work *)
+    (* ltac1:(old new |- assert (old = new) as -> by reflexivity) (Ltac1.of_constr c) (Ltac1.of_constr new_constr) *)
+    ltac1:(old new |- change old with new) (Ltac1.of_constr c) (Ltac1.of_constr new_constr)
+  | context [ dlet (?x1 :: ?x2 :: ?x3 :: ?x4 :: ?x5 :: ?rst) ?f ] =>
+    let prfx := constr:([$x1; $x2; $x3; $x4]) in
+    let sfx := constr:($x5 :: $rst) in
+    let new_constr := constr:(
+      let/d prfx := $prfx in
+      let/d sfx := $sfx in
+      dlet (List.app prfx sfx) $f
+    ) in
+    ltac1:(old new |- assert (old = new) as -> by reflexivity) (Ltac1.of_constr c) (Ltac1.of_constr new_constr)
+  end).
 
 Ltac2 rewrite_lowerable () :=
   repeat (match! goal with
-  | [ |- context [ N.mul _ _ ] ] =>
-    rewrite <- mul_N_spec
-  | [ |- context [ Nat.mul _ _ ] ] =>
-    rewrite <- mul_nat_spec
-  | [ |- context [ append _ _ ] ] =>
-    rewrite <- string_append_spec
-  | [ |- context [ List.app _ _ ] ] =>
-    rewrite <- list_append_spec
-  | [ |- context [ List.length _ ] ] =>
-    rewrite <- list_length_spec
-  | [ |- context [
-    let/d x := (String _ (String _ (String _ (String _ (String _ _))))) in _ ] ] =>
-    rewrite split_string
-  | [ |- context [
-    let/d x := (_ :: _ :: _ :: _ :: _ :: _) in _ ] ] =>
-    rewrite split_list
+  | [|- _ |-- (_, _) ---> ([encode ?c], _) ] =>
+    lower_match_constr c
   end).
 
 (* test *)
+
+Ltac2 rewrite_lowerable_test () :=
+  repeat (match! goal with
+  | [|- ?c = _ ] =>
+    lower_match_constr c
+  end).
 
 Definition test1 (a b: N): N :=
   a * b + N.mul b a.
 
 Goal forall (a b: N), test1 a b = test1 a b.
   intros; unfold test1.
-  rewrite_lowerable ().
+  rewrite_lowerable_test ().
   reflexivity ().
 Qed.
 
@@ -72,7 +78,7 @@ Definition test2 (a b: N): N :=
 
 Goal forall (a b: N), test2 a b = test2 a b.
   intros; unfold test2.
-  rewrite_lowerable ().
+  rewrite_lowerable_test ().
   reflexivity ().
 Qed.
 
@@ -82,9 +88,20 @@ Definition test_split_string (s1 s2: string): string :=
 
 Goal forall (s1 s2: string), test_split_string s1 s2 = test_split_string s1 s2.
   intros; unfold test_split_string.
-  rewrite_lowerable ().
+  rewrite_lowerable_test ().
   reflexivity ().
 Qed.
+
+Goal forall (reg2str1: string -> string -> string) r n str, (let/d anf_tmp := "movq "%string
+in let/d anf_tmp0 := mul_nat 8 n
+in let/d anf_tmp1 := "(%rsp), "%string
+in let/d anf_tmp2 := reg2str1 r str
+in let/d anf_tmp3 := (anf_tmp1 ++ anf_tmp2)%string
+in let/d anf_tmp4 := num2str anf_tmp0 anf_tmp3
+in let/d anf_tmp5 := (anf_tmp ++ anf_tmp4)%string in anf_tmp5) = ""%string.
+  intros.
+  rewrite_lowerable_test ().
+Admitted.
 
 Definition test_split_list (l1 l2: list nat): list nat :=
   let/d l := [1;2;3;4;5;6;7] in
@@ -92,6 +109,6 @@ Definition test_split_list (l1 l2: list nat): list nat :=
 
 Goal forall (l1 l2: list nat), test_split_list l1 l2 = test_split_list l1 l2.
   intros; unfold test_split_list.
-  rewrite_lowerable ().
+  rewrite_lowerable_test ().
   reflexivity ().
 Qed.
