coq/theories/derivations/AsmToStringDerivations.v
@@ -1,23 +1,16 @@
 From impboot Require Import utils.Core.
 From impboot Require Import utils.AppList.
-Require Import impboot.assembly.ASMSyntax.
 Require Import impboot.assembly.ASMToString.
 Require Import impboot.imperative.ImpSyntax.
 Require Import impboot.utils.AppList.
-Require Import impboot.imp2asm.ImpToASMCodegen.
-From impboot Require Import automation.Ltac2Utils.
-From impboot Require Import commons.CompilerUtils.
-From impboot Require Import functional.FunValues.
-From impboot Require Import functional.FunSemantics.
+From impboot.automation Require Import Ltac2Utils ToLowerable ToANF RelCompiler RelCompilerCommons ltac2.UnfoldFix.
+From impboot.commons Require Import CompilerUtils.
+From impboot.functional Require Import FunValues FunSemantics.
 From impboot Require Import assembly.ASMSyntax.
-Require Import impboot.automation.RelCompiler.
-Require Import impboot.automation.ltac2.UnfoldFix.
-Require Import impboot.automation.AutomationLemmas.
-Require Import coqutil.Word.Interface.
-Require Import ZArith.
+From impboot Require Import fp2imp.FpToImpCodegen.
+From Stdlib Require Import ZArith Lia.
 From Stdlib Require Import FunInd.
 From Stdlib Require Import derive.Derive.
-From Stdlib Require Import Lia.
 From Ltac2 Require Import Ltac2.
 
 From impboot Require Import derivations.CompilerUtilsDerivations.
@@ -48,6 +41,7 @@ Derive reg2str1_prog
 Proof.
   time relcompile.
 Qed.
+Time Compute to_funs [reg2str1_prog].
 
 Derive lab_prog
   in ltac2:(relcompile_tpe 'lab_prog 'lab ['num2str])
@@ -55,6 +49,7 @@ Derive lab_prog
 Proof.
   time relcompile.
 Qed.
+Time Compute to_funs [lab_prog].
 
 Derive clean_prog
   in ltac2:(relcompile_tpe 'clean_prog 'clean [])
@@ -62,6 +57,7 @@ Derive clean_prog
 Proof.
   time relcompile.
 Qed.
+Time Compute to_funs [clean_prog].
 
 Derive inst2str_const_prog
   in ltac2:(relcompile_tpe 'inst2str_const_prog 'inst2str_const ['reg2str1; 'string_append; 'N2str])
@@ -69,6 +65,7 @@ Derive inst2str_const_prog
 Proof.
   time relcompile.
 Qed.
+Time Compute to_funs [inst2str_const_prog].
 
 Derive inst2str_mov_prog
   in ltac2:(relcompile_tpe 'inst2str_mov_prog 'inst2str_mov ['reg2str1; 'string_append])
@@ -76,6 +73,7 @@ Derive inst2str_mov_prog
 Proof.
   time relcompile.
 Qed.
+Time Compute to_funs [inst2str_mov_prog].
 
 Derive inst2str_add_prog
   in ltac2:(relcompile_tpe 'inst2str_add_prog 'inst2str_add ['reg2str1; 'string_append])
@@ -83,6 +81,7 @@ Derive inst2str_add_prog
 Proof.
   time relcompile.
 Qed.
+Time Compute to_funs [inst2str_add_prog].
 
 Derive inst2str_sub_prog
   in ltac2:(relcompile_tpe 'inst2str_sub_prog 'inst2str_sub ['reg2str1; 'string_append])
@@ -90,6 +89,7 @@ Derive inst2str_sub_prog
 Proof.
   time relcompile.
 Qed.
+Time Compute to_funs [inst2str_sub_prog].
 
 Derive inst2str_div_prog
   in ltac2:(relcompile_tpe 'inst2str_div_prog 'inst2str_div ['reg2str1; 'string_append])
@@ -97,27 +97,15 @@ Derive inst2str_div_prog
 Proof.
   time relcompile.
 Qed.
+Time Compute to_funs [inst2str_div_prog].
 
-Derive inst2str_jump_always_prog
-  in ltac2:(relcompile_tpe 'inst2str_jump_always_prog 'inst2str_jump_always ['reg2str1; 'string_append; 'lab])
-  as inst2str_jump_always_prog_proof.
+Derive inst2str_jump_prog
+  in ltac2:(relcompile_tpe 'inst2str_jump_prog 'inst2str_jump ['reg2str1; 'string_append; 'lab])
+  as inst2str_jump_prog_proof.
 Proof.
   time relcompile.
 Qed.
-
-Derive inst2str_jump_equal_prog
-  in ltac2:(relcompile_tpe 'inst2str_jump_equal_prog 'inst2str_jump_equal ['reg2str1; 'string_append; 'lab])
-  as inst2str_jump_equal_prog_proof.
-Proof.
-  time relcompile.
-Qed.
-
-Derive inst2str_jump_less_prog
-  in ltac2:(relcompile_tpe 'inst2str_jump_less_prog 'inst2str_jump_less ['reg2str1; 'string_append; 'lab])
-  as inst2str_jump_less_prog_proof.
-Proof.
-  time relcompile.
-Qed.
+Time Compute to_funs [inst2str_jump_prog].
 
 Derive inst2str_call_prog
   in ltac2:(relcompile_tpe 'inst2str_call_prog 'inst2str_call ['reg2str1; 'string_append; 'lab])
@@ -125,6 +113,7 @@ Derive inst2str_call_prog
 Proof.
   time relcompile.
 Qed.
+Time Compute to_funs [inst2str_call_prog].
 
 Derive inst2str_ret_prog
   in ltac2:(relcompile_tpe 'inst2str_ret_prog 'inst2str_ret ['reg2str1; 'string_append; 'lab])
@@ -132,6 +121,7 @@ Derive inst2str_ret_prog
 Proof.
   time relcompile.
 Qed.
+Time Compute to_funs [inst2str_ret_prog].
 
 Derive inst2str_pop_prog
   in ltac2:(relcompile_tpe 'inst2str_pop_prog 'inst2str_pop ['reg2str1; 'string_append; 'lab])
@@ -139,6 +129,7 @@ Derive inst2str_pop_prog
 Proof.
   time relcompile.
 Qed.
+Time Compute to_funs [inst2str_pop_prog].
 
 Derive inst2str_push_prog
   in ltac2:(relcompile_tpe 'inst2str_push_prog 'inst2str_push ['reg2str1; 'string_append; 'lab])
@@ -146,6 +137,7 @@ Derive inst2str_push_prog
 Proof.
   time relcompile.
 Qed.
+Time Compute to_funs [inst2str_push_prog].
 
 Derive inst2str_load_rsp_prog
   in ltac2:(relcompile_tpe 'inst2str_load_rsp_prog 'inst2str_load_rsp ['reg2str1; 'string_append; 'lab; 'mul_nat; 'num2str])
@@ -153,6 +145,7 @@ Derive inst2str_load_rsp_prog
 Proof.
   time relcompile.
 Qed.
+Time Compute to_funs [inst2str_load_rsp_prog].
 
 Derive inst2str_store_rsp_prog
   in ltac2:(relcompile_tpe 'inst2str_store_rsp_prog 'inst2str_store_rsp ['reg2str1; 'string_append; 'lab; 'mul_nat; 'num2str])
@@ -160,6 +153,7 @@ Derive inst2str_store_rsp_prog
 Proof.
   time relcompile.
 Qed.
+Time Compute to_funs [inst2str_store_rsp_prog].
 
 Derive inst2str_add_rsp_prog
   in ltac2:(relcompile_tpe 'inst2str_add_rsp_prog 'inst2str_add_rsp ['reg2str1; 'string_append; 'lab; 'mul_nat; 'num2str])
@@ -167,6 +161,7 @@ Derive inst2str_add_rsp_prog
 Proof.
   time relcompile.
 Qed.
+Time Compute to_funs [inst2str_add_rsp_prog].
 
 Derive inst2str_sub_rsp_prog
   in ltac2:(relcompile_tpe 'inst2str_sub_rsp_prog 'inst2str_sub_rsp ['reg2str1; 'string_append; 'lab; 'mul_nat; 'num2str])
@@ -174,6 +169,7 @@ Derive inst2str_sub_rsp_prog
 Proof.
   time relcompile.
 Qed.
+Time Compute to_funs [inst2str_sub_rsp_prog].
 
 Derive inst2str_store_prog
   in ltac2:(relcompile_tpe 'inst2str_store_prog 'inst2str_store ['reg2str1; 'string_append; 'lab; 'mul_nat; 'num2str; 'N2str])
@@ -181,6 +177,7 @@ Derive inst2str_store_prog
 Proof.
   time relcompile.
 Qed.
+Time Compute to_funs [inst2str_store_prog].
 
 Derive inst2str_load_prog
   in ltac2:(relcompile_tpe 'inst2str_load_prog 'inst2str_load ['reg2str1; 'string_append; 'lab; 'mul_nat; 'num2str; 'N2str])
@@ -188,6 +185,7 @@ Derive inst2str_load_prog
 Proof.
   time relcompile.
 Qed.
+Time Compute to_funs [inst2str_load_prog].
 
 Derive inst2str_getchar1_prog
   in ltac2:(relcompile_tpe 'inst2str_getchar1_prog 'inst2str_getchar1 ['reg2str1; 'string_append; 'lab; 'mul_nat; 'num2str; 'N2str])
@@ -195,6 +193,7 @@ Derive inst2str_getchar1_prog
 Proof.
   time relcompile.
 Qed.
+Time Compute to_funs [inst2str_getchar1_prog].
 
 Derive inst2str_putchar_prog
   in ltac2:(relcompile_tpe 'inst2str_putchar_prog 'inst2str_putchar ['reg2str1; 'string_append; 'lab; 'mul_nat; 'num2str; 'N2str])
@@ -202,6 +201,7 @@ Derive inst2str_putchar_prog
 Proof.
   time relcompile.
 Qed.
+Time Compute to_funs [inst2str_putchar_prog].
 
 Derive inst2str_exit_prog
   in ltac2:(relcompile_tpe 'inst2str_exit_prog 'inst2str_exit ['reg2str1; 'string_append; 'lab; 'mul_nat; 'num2str; 'N2str])
@@ -209,6 +209,7 @@ Derive inst2str_exit_prog
 Proof.
   time relcompile.
 Qed.
+Time Compute to_funs [inst2str_exit_prog].
 
 Derive inst2str_comment_prog
   in ltac2:(relcompile_tpe 'inst2str_comment_prog 'inst2str_comment ['reg2str1; 'string_append; 'lab; 'mul_nat; 'num2str; 'N2str; 'clean])
@@ -216,14 +217,16 @@ Derive inst2str_comment_prog
 Proof.
   time relcompile.
 Qed.
+Time Compute to_funs [inst2str_comment_prog].
 
 Derive inst2str_prog
-  in ltac2:(relcompile_tpe 'inst2str_prog 'inst2str ['inst2str_const; 'inst2str_mov; 'inst2str_add; 'inst2str_sub; 'inst2str_div; 'inst2str_jump_always; 'inst2str_jump_equal; 'inst2str_jump_less; 'inst2str_call; 'inst2str_ret; 'inst2str_pop; 'inst2str_push; 'inst2str_load_rsp; 'inst2str_store_rsp; 'inst2str_add_rsp; 'inst2str_sub_rsp; 'inst2str_store; 'inst2str_load; 'inst2str_getchar1; 'inst2str_putchar; 'inst2str_exit; 'inst2str_comment])
+  in ltac2:(relcompile_tpe 'inst2str_prog 'inst2str ['inst2str_const; 'inst2str_mov; 'inst2str_add; 'inst2str_sub; 'inst2str_div; 'inst2str_jump; 'inst2str_call; 'inst2str_ret; 'inst2str_pop; 'inst2str_push; 'inst2str_load_rsp; 'inst2str_store_rsp; 'inst2str_add_rsp; 'inst2str_sub_rsp; 'inst2str_store; 'inst2str_load; 'inst2str_getchar1; 'inst2str_putchar; 'inst2str_exit; 'inst2str_comment])
   as inst2str_prog_proof.
 Proof.
   (* ltac1:(timeout 28 ltac2:(relcompile)). *)
   time relcompile.
 Qed.
+Time Compute to_funs [inst2str_prog].
 
 Derive instrs2str_prog
   in ltac2:(relcompile_tpe 'instrs2str_prog 'instrs2str ['lab; 'inst2str])
@@ -231,6 +234,7 @@ Derive instrs2str_prog
 Proof.
   time relcompile.
 Qed.
+Time Compute to_funs [instrs2str_prog].
 
 Theorem concat_strings_equation: ltac2:(unfold_fix_type '@concat_strings).
 Proof. unfold_fix_proof '@concat_strings. Qed.
@@ -240,34 +244,113 @@ Derive concat_strings_prog
 Proof.
   time relcompile.
 Qed.
+Time Compute to_funs [concat_strings_prog].
 
-Derive asm2str_header1_prog
-  in ltac2:(relcompile_tpe 'asm2str_header1_prog 'asm2str_header1 ['instrs2str; 'concat_strings; '@list_append; 'string_append])
-  as asm2str_header1_prog_proof.
+Derive asm2str1_prog
+  in ltac2:(relcompile_tpe 'asm2str1_prog 'asm2str1 ['instrs2str; 'concat_strings; '@list_append; 'string_append])
+  as asm2str1_prog_proof.
 Proof.
   time relcompile.
 Qed.
+Time Compute to_funs [asm2str1_prog].
 
-Derive asm2str_header2_prog
-  in ltac2:(relcompile_tpe 'asm2str_header2_prog 'asm2str_header2 ['instrs2str; 'concat_strings; '@list_append; 'string_append])
-  as asm2str_header2_prog_proof.
+Derive asm2str2_prog
+  in ltac2:(relcompile_tpe 'asm2str2_prog 'asm2str2 ['instrs2str; 'concat_strings; '@list_append; 'string_append])
+  as asm2str2_prog_proof.
 Proof.
   time relcompile.
 Qed.
+Time Compute to_funs [asm2str2_prog].
 
-Derive asm2str_header3_prog
-  in ltac2:(relcompile_tpe 'asm2str_header3_prog 'asm2str_header3 ['instrs2str; 'concat_strings; '@list_append; 'string_append])
-  as asm2str_header3_prog_proof.
+Derive asm2str3_prog
+  in ltac2:(relcompile_tpe 'asm2str3_prog 'asm2str3 ['instrs2str; 'concat_strings; '@list_append; 'string_append])
+  as asm2str3_prog_proof.
 Proof.
   time relcompile.
 Qed.
+Time Compute to_funs [asm2str3_prog].
+
+Derive asm2str4_prog
+  in ltac2:(relcompile_tpe 'asm2str4_prog 'asm2str4 ['instrs2str; 'concat_strings; '@list_append; 'string_append])
+  as asm2str4_prog_proof.
+Proof.
+  time relcompile.
+Qed.
+Time Compute to_funs [asm2str4_prog].
+
+Derive asm2str5_prog
+  in ltac2:(relcompile_tpe 'asm2str5_prog 'asm2str5 ['instrs2str; 'concat_strings; '@list_append; 'string_append])
+  as asm2str5_prog_proof.
+Proof.
+  time relcompile.
+Qed.
+Time Compute to_funs [asm2str5_prog].
+
+Derive asm2str6_prog
+  in ltac2:(relcompile_tpe 'asm2str6_prog 'asm2str6 ['instrs2str; 'concat_strings; '@list_append; 'string_append])
+  as asm2str6_prog_proof.
+Proof.
+  time relcompile.
+Qed.
+Time Compute to_funs [asm2str6_prog].
+
+Derive asm2str7_prog
+  in ltac2:(relcompile_tpe 'asm2str7_prog 'asm2str7 ['instrs2str; 'concat_strings; '@list_append; 'string_append])
+  as asm2str7_prog_proof.
+Proof.
+  time relcompile.
+Qed.
+Time Compute to_funs [asm2str7_prog].
+
+Derive asm2str8_prog
+  in ltac2:(relcompile_tpe 'asm2str8_prog 'asm2str8 ['instrs2str; 'concat_strings; '@list_append; 'string_append])
+  as asm2str8_prog_proof.
+Proof.
+  time relcompile.
+Qed.
+Time Compute to_funs [asm2str8_prog].
+
+Derive asm2str9_prog
+  in ltac2:(relcompile_tpe 'asm2str9_prog 'asm2str9 ['instrs2str; 'concat_strings; '@list_append; 'string_append])
+  as asm2str9_prog_proof.
+Proof.
+  time relcompile.
+Qed.
+Time Compute to_funs [asm2str9_prog].
+
+Derive asm2str10_prog
+  in ltac2:(relcompile_tpe 'asm2str10_prog 'asm2str10 ['instrs2str; 'concat_strings; '@list_append; 'string_append])
+  as asm2str10_prog_proof.
+Proof.
+  time relcompile.
+Qed.
+Time Compute to_funs [asm2str10_prog].
+
+Derive asm2str11_prog
+  in ltac2:(relcompile_tpe 'asm2str11_prog 'asm2str11 ['instrs2str; 'concat_strings; '@list_append; 'string_append])
+  as asm2str11_prog_proof.
+Proof.
+  time relcompile.
+Qed.
+Time Compute to_funs [asm2str11_prog].
+
+Derive asm2str12_prog
+  in ltac2:(relcompile_tpe 'asm2str12_prog 'asm2str12 ['instrs2str; 'concat_strings; '@list_append; 'string_append])
+  as asm2str12_prog_proof.
+Proof.
+  time relcompile.
+Qed.
+Time Compute to_funs [asm2str12_prog].
 
 Derive asm2str_prog
-  in ltac2:(relcompile_tpe 'asm2str_prog 'asm2str ['instrs2str; 'concat_strings; '@list_append; 'string_append; 'asm2str_header1; 'asm2str_header2; 'asm2str_header3])
+  in ltac2:(relcompile_tpe 'asm2str_prog 'asm2str
+    ['instrs2str; 'concat_strings; '@list_append; 'string_append;
+    'asm2str1; 'asm2str2; 'asm2str3; 'asm2str4; 'asm2str5; 'asm2str6; 'asm2str7; 'asm2str8; 'asm2str9; 'asm2str10; 'asm2str11; 'asm2str12])
   as asm2str_prog_proof.
 Proof.
   time relcompile.
 Qed.
+Time Compute to_funs [asm2str_prog].
 
 Definition ASMToString_funs := [
   reg2str1_prog;
@@ -278,9 +361,7 @@ Definition ASMToString_funs := [
   inst2str_add_prog;
   inst2str_sub_prog;
   inst2str_div_prog;
-  inst2str_jump_always_prog;
-  inst2str_jump_equal_prog;
-  inst2str_jump_less_prog;
+  inst2str_jump_prog;
   inst2str_call_prog;
   inst2str_ret_prog;
   inst2str_pop_prog;
@@ -298,9 +379,18 @@ Definition ASMToString_funs := [
   inst2str_prog;
   instrs2str_prog;
   concat_strings_prog;
-  asm2str_header1_prog;
-  asm2str_header2_prog;
-  asm2str_header3_prog;
+  asm2str1_prog;
+  asm2str2_prog;
+  asm2str3_prog;
+  asm2str4_prog;
+  asm2str5_prog;
+  asm2str6_prog;
+  asm2str7_prog;
+  asm2str8_prog;
+  asm2str9_prog;
+  asm2str10_prog;
+  asm2str11_prog;
+  asm2str12_prog;
   asm2str_prog
 ].
 
@@ -353,29 +443,36 @@ Proof.
   assert_eval_app_by 'inst2str_add 'inst2str_add_prog_proof 'Hlookup_fun 5.
   assert_eval_app_by 'inst2str_sub 'inst2str_sub_prog_proof 'Hlookup_fun 6.
   assert_eval_app_by 'inst2str_div 'inst2str_div_prog_proof 'Hlookup_fun 7.
-  assert_eval_app_by 'inst2str_jump_always 'inst2str_jump_always_prog_proof 'Hlookup_fun 8.
-  assert_eval_app_by 'inst2str_jump_equal 'inst2str_jump_equal_prog_proof 'Hlookup_fun 9.
-  assert_eval_app_by 'inst2str_jump_less 'inst2str_jump_less_prog_proof 'Hlookup_fun 10.
-  assert_eval_app_by 'inst2str_call 'inst2str_call_prog_proof 'Hlookup_fun 11.
-  assert_eval_app_by 'inst2str_ret 'inst2str_ret_prog_proof 'Hlookup_fun 12.
-  assert_eval_app_by 'inst2str_pop 'inst2str_pop_prog_proof 'Hlookup_fun 13.
-  assert_eval_app_by 'inst2str_push 'inst2str_push_prog_proof 'Hlookup_fun 14.
-  assert_eval_app_by 'inst2str_load_rsp 'inst2str_load_rsp_prog_proof 'Hlookup_fun 15.
-  assert_eval_app_by 'inst2str_store_rsp 'inst2str_store_rsp_prog_proof 'Hlookup_fun 16.
-  assert_eval_app_by 'inst2str_add_rsp 'inst2str_add_rsp_prog_proof 'Hlookup_fun 17.
-  assert_eval_app_by 'inst2str_sub_rsp 'inst2str_sub_rsp_prog_proof 'Hlookup_fun 18.
-  assert_eval_app_by 'inst2str_store 'inst2str_store_prog_proof 'Hlookup_fun 19.
-  assert_eval_app_by 'inst2str_load 'inst2str_load_prog_proof 'Hlookup_fun 20.
-  assert_eval_app_by 'inst2str_getchar1 'inst2str_getchar1_prog_proof 'Hlookup_fun 21.
-  assert_eval_app_by 'inst2str_putchar 'inst2str_putchar_prog_proof 'Hlookup_fun 22.
-  assert_eval_app_by 'inst2str_exit 'inst2str_exit_prog_proof 'Hlookup_fun 23.
-  assert_eval_app_by 'inst2str_comment 'inst2str_comment_prog_proof 'Hlookup_fun 24.
-  assert_eval_app_by 'inst2str 'inst2str_prog_proof 'Hlookup_fun 25.
-  assert_eval_app_by 'instrs2str 'instrs2str_prog_proof 'Hlookup_fun 26.
-  assert_eval_app_by 'concat_strings 'concat_strings_prog_proof 'Hlookup_fun 27.
-  assert_eval_app_by 'asm2str_header1 'asm2str_header1_prog_proof 'Hlookup_fun 28.
-  assert_eval_app_by 'asm2str_header2 'asm2str_header2_prog_proof 'Hlookup_fun 29.
-  assert_eval_app_by 'asm2str_header3 'asm2str_header3_prog_proof 'Hlookup_fun 30.
-  assert_eval_app_by 'asm2str 'asm2str_prog_proof 'Hlookup_fun 31.
+  assert_eval_app_by 'inst2str_jump 'inst2str_jump_prog_proof 'Hlookup_fun 8.
+  assert_eval_app_by 'inst2str_call 'inst2str_call_prog_proof 'Hlookup_fun 9.
+  assert_eval_app_by 'inst2str_ret 'inst2str_ret_prog_proof 'Hlookup_fun 10.
+  assert_eval_app_by 'inst2str_pop 'inst2str_pop_prog_proof 'Hlookup_fun 11.
+  assert_eval_app_by 'inst2str_push 'inst2str_push_prog_proof 'Hlookup_fun 12.
+  assert_eval_app_by 'inst2str_load_rsp 'inst2str_load_rsp_prog_proof 'Hlookup_fun 13.
+  assert_eval_app_by 'inst2str_store_rsp 'inst2str_store_rsp_prog_proof 'Hlookup_fun 14.
+  assert_eval_app_by 'inst2str_add_rsp 'inst2str_add_rsp_prog_proof 'Hlookup_fun 15.
+  assert_eval_app_by 'inst2str_sub_rsp 'inst2str_sub_rsp_prog_proof 'Hlookup_fun 16.
+  assert_eval_app_by 'inst2str_store 'inst2str_store_prog_proof 'Hlookup_fun 17.
+  assert_eval_app_by 'inst2str_load 'inst2str_load_prog_proof 'Hlookup_fun 18.
+  assert_eval_app_by 'inst2str_getchar1 'inst2str_getchar1_prog_proof 'Hlookup_fun 19.
+  assert_eval_app_by 'inst2str_putchar 'inst2str_putchar_prog_proof 'Hlookup_fun 20.
+  assert_eval_app_by 'inst2str_exit 'inst2str_exit_prog_proof 'Hlookup_fun 21.
+  assert_eval_app_by 'inst2str_comment 'inst2str_comment_prog_proof 'Hlookup_fun 22.
+  assert_eval_app_by 'inst2str 'inst2str_prog_proof 'Hlookup_fun 23.
+  assert_eval_app_by 'instrs2str 'instrs2str_prog_proof 'Hlookup_fun 24.
+  assert_eval_app_by 'concat_strings 'concat_strings_prog_proof 'Hlookup_fun 25.
+  assert_eval_app_by 'asm2str1 'asm2str1_prog_proof 'Hlookup_fun 26.
+  assert_eval_app_by 'asm2str2 'asm2str2_prog_proof 'Hlookup_fun 27.
+  assert_eval_app_by 'asm2str3 'asm2str3_prog_proof 'Hlookup_fun 28.
+  assert_eval_app_by 'asm2str4 'asm2str4_prog_proof 'Hlookup_fun 29.
+  assert_eval_app_by 'asm2str5 'asm2str5_prog_proof 'Hlookup_fun 30.
+  assert_eval_app_by 'asm2str6 'asm2str6_prog_proof 'Hlookup_fun 31.
+  assert_eval_app_by 'asm2str7 'asm2str7_prog_proof 'Hlookup_fun 32.
+  assert_eval_app_by 'asm2str8 'asm2str8_prog_proof 'Hlookup_fun 33.
+  assert_eval_app_by 'asm2str9 'asm2str9_prog_proof 'Hlookup_fun 34.
+  assert_eval_app_by 'asm2str10 'asm2str10_prog_proof 'Hlookup_fun 35.
+  assert_eval_app_by 'asm2str11 'asm2str11_prog_proof 'Hlookup_fun 36.
+  assert_eval_app_by 'asm2str12 'asm2str12_prog_proof 'Hlookup_fun 37.
+  assert_eval_app_by 'asm2str 'asm2str_prog_proof 'Hlookup_fun 38.
   eauto.
 Qed.
