coq/theories/derivations/CompilerUtilsDerivations.v
@@ -13,6 +13,7 @@ From impboot Require Import functional.FunSemantics.
 Require Import impboot.automation.RelCompiler.
 Require Import impboot.automation.ltac2.UnfoldFix.
 Require Import impboot.automation.AutomationLemmas.
+From impboot Require Import fp2imp.FpToImpCodegen.
 Require Import coqutil.Word.Interface.
 Require Import ZArith.
 From Stdlib Require Import FunInd.
@@ -27,6 +28,7 @@ Proof.
   time relcompile.
   ltac1:(lia).
 Qed.
+Time Compute to_funs [nat_modulo_prog].
 
 Derive N_modulo_prog
   in ltac2:(relcompile_tpe 'N_modulo_prog 'N_modulo ['mul_N]) 
@@ -35,6 +37,7 @@ Proof.
   time relcompile.
   ltac1:(lia).
 Qed.
+Time Compute to_funs [nat_modulo_prog].
 
 Theorem string_append_equation: ltac2:(unfold_fix_type '@string_append).
 Proof. unfold_fix_proof '@string_append. Qed.
@@ -44,6 +47,7 @@ Derive string_append_prog
 Proof.
   time relcompile.
 Qed.
+Time Compute to_funs [nat_modulo_prog].
 
 Theorem num2str_f_equation: ltac2:(unfold_fix_type '@num2str_f).
 Proof. unfold_fix_proof '@num2str_f. Qed.
@@ -56,6 +60,7 @@ Proof.
   all: ltac1:(try lia).
   all: subst; specialize nat_modulo_le with (n := n) (m := 10); ltac1:(lia).
 Qed.
+Time Compute to_funs [num2str_f_prog].
 
 Derive num2str_prog
   in ltac2:(relcompile_tpe 'num2str_prog 'num2str ['num2str_f])
@@ -63,6 +68,7 @@ Derive num2str_prog
 Proof.
   time relcompile.
 Qed.
+Time Compute to_funs [num2str_prog].
 
 Theorem N2str_f_equation: ltac2:(unfold_fix_type '@N2str_f).
 Proof. unfold_fix_proof '@N2str_f. Qed.
@@ -76,6 +82,7 @@ Proof.
   all: rewrite ?N.ltb_lt in *; ltac1:(try lia).
   all: subst; specialize N_modulo_le with (n := n) (m := 10%N) as ?; ltac1:(try lia).
 Qed.
+Time Compute to_funs [N2str_f_prog].
 
 Derive N2str_prog
   in ltac2:(relcompile_tpe 'N2str_prog 'N2str ['N2str_f])
@@ -84,6 +91,7 @@ Proof.
   time relcompile.
   ltac1:(try lia).
 Qed.
+Time Compute to_funs [N2str_prog].
 
 Theorem list_length_equation: ltac2:(unfold_fix_type '@list_length).
 Proof. unfold_fix_proof '@list_length. Qed.
@@ -94,6 +102,7 @@ Derive list_length_prog
 Proof.
   time relcompile.
 Qed.
+Time Compute to_funs [list_length_prog].
 
 Theorem list_append_equation: ltac2:(unfold_fix_type '@list_append).
 Proof. unfold_fix_proof '@list_append. Qed.
@@ -104,6 +113,7 @@ Derive list_append_prog
 Proof.
   time relcompile.
 Qed.
+Time Compute to_funs [list_append_prog].
 
 Theorem flatten_equation: ltac2:(unfold_fix_type '@flatten).
 Proof. unfold_fix_proof '@flatten. Qed.
@@ -114,6 +124,7 @@ Derive flatten_prog
 Proof.
   time relcompile.
 Qed.
+Time Compute to_funs [flatten_prog].
 
 Theorem app_list_length_equation: ltac2:(unfold_fix_type '@app_list_length).
 Proof. unfold_fix_proof '@app_list_length. Qed.
@@ -124,6 +135,7 @@ Derive app_list_length_prog
 Proof.
   time relcompile.
 Qed.
+Time Compute to_funs [app_list_length_prog].
 
 Theorem mul_nat_equation: ltac2:(unfold_fix_type '@mul_nat).
 Proof. unfold_fix_proof '@mul_nat. Qed.
@@ -133,6 +145,7 @@ Derive mul_nat_prog
 Proof.
   time relcompile.
 Qed.
+Time Compute to_funs [mul_nat_prog].
 
 Theorem mul_N_f_equation: ltac2:(unfold_fix_type '@mul_N_f).
 Proof. unfold_fix_proof '@mul_N_f. Qed.
@@ -142,6 +155,7 @@ Derive mul_N_f_prog
 Proof.
   time relcompile.
 Qed.
+Time Compute to_funs [mul_N_f_prog].
 
 Derive mul_N_prog
   in ltac2:(relcompile_tpe 'mul_N_prog 'mul_N ['mul_N_f])
@@ -149,6 +163,7 @@ Derive mul_N_prog
 Proof.
   time relcompile.
 Qed.
+Time Compute to_funs [mul_N_prog].
 
 Definition CompilerUtils_funs := [
   mul_nat_prog;
